Find dependencies, type arg names were reversed, concretization

extraction/theories/MidlangExtract.v
@@ -6,6 +6,8 @@ From ConCert.Extraction Require Import Certified.
 From Coq Require Import Arith.
 From Coq Require Import Ascii.
 From Coq Require Import List.
+From Coq Require Import NArith.
+From Coq Require Import PArith.
 From Coq Require Import String.
 
 From MetaCoq.SafeChecker Require Import PCUICSafeChecker SafeTemplateChecker.
@@ -17,6 +19,7 @@ Module PT := MetaCoq.PCUIC.PCUICTyping.
 Module T2P := MetaCoq.PCUIC.TemplateToPCUIC.
 Module E := MetaCoq.Erasure.EAst.
 Module T := MetaCoq.Template.Ast.
+Module TUtil := MetaCoq.Template.AstUtils.
 Module EF := MetaCoq.Erasure.SafeErasureFunction.
 
 Import ListNotations.
@@ -31,7 +34,7 @@ Module Ex.
 
   Inductive global_decl :=
   | ConstantDecl : constant_body -> global_decl
-  | InductiveDecl : P.mutual_inductive_body -> global_decl.
+  | InductiveDecl : P.mutual_inductive_body -> E.mutual_inductive_body -> global_decl.
 
   Definition global_env := list (kername * global_decl).
 
@@ -135,7 +138,7 @@ Definition append_indent : PrettyPrinter unit :=
 Definition append_nl_and_indent : PrettyPrinter unit :=
   append_nl;; append_indent.
 
-Definition replace_char (orig : Ascii.ascii) (new : Ascii.ascii) : string -> string :=
+Definition replace_char (orig : ascii) (new : ascii) : string -> string :=
   fix f s :=
     match s with
     | EmptyString => EmptyString
@@ -143,6 +146,16 @@ Definition replace_char (orig : Ascii.ascii) (new : Ascii.ascii) : string -> str
                       String new (f s)
                     else
                       String c (f s)
+    end.
+
+Definition remove_char (c : ascii) : string -> string :=
+  fix f s :=
+    match s with
+    | EmptyString => EmptyString
+    | String c' s => if (c' =? c)%char then
+                       f s
+                     else
+                       String c' (f s)
     end.
 
 Definition last_index_of (c : ascii) (s : string) : option nat :=
@@ -180,7 +193,7 @@ Definition uncapitalize (s : string) : string :=
   | String c s => String (to_lower c) s
   end.
 
-Definition printable_kername (name : kername) : string :=
+Definition unqual_kername (name : kername) : string :=
   match last_index_of "." name with
   | Some n => substring (S n) (length name) name
   | None => name
@@ -200,24 +213,21 @@ Section FixExEnv.
 
 Context (Σ : Ex.global_env).
 
+Definition get_fun_name (name : kername) : string :=
+  uncapitalize (replace_char "." "_" name).
+
 Definition get_ty_name (name : kername) : string :=
-  capitalize (printable_kername name).
+  capitalize (replace_char "." "_" name).
 
-Definition print_ty_name (name : kername) : PrettyPrinter unit :=
-  append (get_ty_name name).
-
-Definition print_ctor_name (name : ident) : PrettyPrinter unit :=
-  append (capitalize name).
+Definition get_ctor_name (name : ident) : string :=
+  capitalize name.
 
 Definition get_ty_arg_name (name : ident) : ident :=
   uncapitalize name.
 
-Definition print_type_arg_name (name : ident) : PrettyPrinter unit :=
-  append (get_ty_arg_name name).
-
 Definition lookup_mind (name : kername) : option P.mutual_inductive_body :=
   match Ex.lookup_env Σ name with
-  | Some (Ex.InductiveDecl mind) => Some mind
+  | Some (Ex.InductiveDecl mind _) => Some mind
   | _ => None
   end.
 
@@ -237,7 +247,7 @@ Definition print_ind_ctor (ind : inductive) (i : nat) : PrettyPrinter unit :=
   oib <- lookup_ind_decl ind;;
   match nth_error (P.ind_ctors oib) i with
   | Some (name, _, _) =>
-    print_ctor_name name
+    append (get_ctor_name name)
     (*append (replace_char "." "_" (inductive_mind ind) ++ "_" ++ name)*)
   | None =>
     printer_fail (inductive_mind ind ++ " does not have a ctor " ++ string_of_nat i)
@@ -296,11 +306,11 @@ Definition fresh (name : ident) (used : list ident) : ident :=
   else
     name.
 
-Definition fresh_name (name : name) (Γ : list ident) : PrettyPrinter ident :=
+Definition fresh_ident (name : name) (Γ : list ident) : PrettyPrinter ident :=
   used_names <- get_used_names;;
   match name with
   | nAnon => ret (fresh "_x" (Γ ++ used_names))
-  | nNamed name => ret (fresh name (Γ ++ used_names))
+  | nNamed name => ret (fresh (remove_char "'" name) (Γ ++ used_names))
   end.
 
 Definition fresh_ty_arg_name (name : name) (Γ : list ident) : PrettyPrinter ident :=
@@ -323,8 +333,6 @@ Definition parenthesize_ty_app_arg (t : term) : bool :=
   | _ => false
   end.
 
-Quote Recursively Definition asdawd := fold_left.
-
 Fixpoint print_type (Γ : list (option ident)) (t : term) : PrettyPrinter unit :=
   match t with
   | tRel n =>
@@ -335,7 +343,7 @@ Fixpoint print_type (Γ : list (option ident)) (t : term) : PrettyPrinter unit :
     | None =>
       printer_fail ("unbound tRel " ++ string_of_nat n)
     end
-  | tInd ind _ => print_ty_name (inductive_mind ind)
+  | tInd ind _ => append (get_ty_name (inductive_mind ind))
   | tProd name (tSort _) cod =>
     (* Midlang is implicitly generalized over type args *)
     let or_empty o :=
@@ -376,7 +384,7 @@ Definition print_define_term
   let fix print_decompose Γ t :=
       match t with
       | tLambda arg_name t =>
-        arg_name <- fresh_name arg_name Γ;;
+        arg_name <- fresh_ident arg_name Γ;;
         append (" " ++ arg_name);;
         print_decompose (arg_name :: Γ) t
       | _ =>
@@ -405,7 +413,7 @@ Fixpoint print_term (Γ : list ident) (t : term) : PrettyPrinter unit :=
   | tLambda name t =>
     append "\";;
 
-    name <- fresh_name name Γ;;
+    name <- fresh_ident name Γ;;
     append name;;
     append " -> ";;
     print_term (name :: Γ) t
@@ -419,7 +427,7 @@ Fixpoint print_term (Γ : list ident) (t : term) : PrettyPrinter unit :=
 
     let print_and_add_one Γ name value :=
         append_nl_and_indent;;
-        name <- fresh_name name Γ;;
+        name <- fresh_ident name Γ;;
         (* We will define this name to make sure we don't reuse it
            until the let is all over. Midlang does not allow shadowing. *)
         push_use name;;
@@ -471,7 +479,7 @@ Fixpoint print_term (Γ : list ident) (t : term) : PrettyPrinter unit :=
     append " ";;
     print_parenthesized (parenthesize_app_arg arg) (print_term Γ arg)
 
-  | tConst name => append (printable_kername name)
+  | tConst name => append (get_fun_name name)
   | tConstruct ind i => print_ind_ctor ind i
 
   | tCase (ind, _) discriminee branches =>
@@ -495,7 +503,7 @@ Fixpoint print_term (Γ : list ident) (t : term) : PrettyPrinter unit :=
          ctor_indent <- get_indent;;
          push_indent (ctor_indent + indent_size);;
 
-         print_ctor_name ctor_name;;
+         append (get_ctor_name ctor_name);;
 
          (fix print_branch (n : nat) (Γ : list ident) (t : term) {struct t} :=
             match n with
@@ -507,7 +515,7 @@ Fixpoint print_term (Γ : list ident) (t : term) : PrettyPrinter unit :=
             | S n =>
               match t with
               | tLambda name t =>
-                name <- fresh_name name Γ;;
+                name <- fresh_ident name Γ;;
                 append (" " ++ name);;
                 print_branch n (name :: Γ) t
 
@@ -531,7 +539,7 @@ Fixpoint print_term (Γ : list ident) (t : term) : PrettyPrinter unit :=
 
     (* Add names of fixes to context *)
     Γ <- monad_fold_left
-           (fun Γ d => name <- fresh_name (dname d) Γ;;
+           (fun Γ d => name <- fresh_ident (dname d) Γ;;
                        ret (name :: Γ)) mfix Γ;;
     let names := rev (firstn (List.length mfix) Γ) in
 
@@ -565,27 +573,32 @@ Fixpoint print_term (Γ : list ident) (t : term) : PrettyPrinter unit :=
   | tCoFix _ _ => printer_fail "Cannot handle cofix"
   end.
 
-Definition print_constant_body (name : kername) (cst : Ex.constant_body) : PrettyPrinter unit :=
+Definition print_constant_body
+           (name : kername)
+           (cst : Ex.constant_body) : PrettyPrinter string :=
   name_col <- get_current_line_length;;
 
   push_indent name_col;;
 
   let (type, body) := cst in
 
-  append (printable_kername name);;
+  let ml_name := get_fun_name name in
+  (*
+  append ml_name;;
   append " : ";;
-  print_type [] type;;
+  print_type [] type;;*)
 
   match body with
   | None => ret tt
   | Some body =>
-    append_nl_and_indent;;
-    let name := printable_kername name in
+    let name := get_fun_name name in
     push_use name;;
     print_define_term [] name body print_term
   end;;
 
-  pop_indent.
+  pop_indent;;
+
+  ret ml_name.
 
 Quote Recursively Definition foo := (None : option nat)%nat.
 
@@ -629,7 +642,7 @@ Definition print_ind_ctor_definition
            (ty : P.term)
            (nparams : nat)
            (arity : nat) : PrettyPrinter unit :=
-  print_ctor_name name;;
+  append (get_ctor_name name);;
   tys <- decompose_ind_ctor nparams arity ty;;
 
   (fix f (Γ : list (option ident)) (tys : list P.term) :=
@@ -644,14 +657,14 @@ Definition print_ind_ctor_definition
 Local Open Scope string.
 Definition print_mutual_inductive_body
            (name : kername)
-           (mib : P.mutual_inductive_body) : PrettyPrinter unit :=
+           (mib : P.mutual_inductive_body) : PrettyPrinter (list (kername * string)) :=
   col <- get_current_line_length;;
   push_indent col;;
 
   let qualifier := kername_qualifier name in
 
   (* make context that has mutual inductive bodies *)
-  let Γ := rev_map (fun oib => get_ty_name (ind_name oib)) (ind_bodies mib) in
+  let Γ := rev_map (fun oib => get_ty_name (qualifier ++ "." ++ ind_name oib)) (ind_bodies mib) in
   (* add parameters *)
   Γ <- monad_fold_left
          (fun Γ d =>
@@ -664,22 +677,25 @@ Definition print_mutual_inductive_body
             | t => printer_fail "can only handle parameters of type sort"
             end;;
             name <- fresh_ty_arg_name (decl_name d) Γ;;
-            ret (name :: Γ)) (ind_params mib) Γ;;
+            ret (name :: Γ)) (rev (ind_params mib)) Γ;;
 
   let ty_arg_names := rev (firstn (List.length (ind_params mib)) Γ) in
 
+  names <-
   (fix print_ind_bodies
        (l : list P.one_inductive_body)
-       (first : bool) :=
+       (first : bool)
+       (names : list (kername * string)) :=
      match l with
-     | [] => ret tt
+     | [] => ret names
      | oib :: l =>
 
        (if first then ret tt else append_nl_and_indent);;
 
        append "type ";;
        let ind_name := qualifier ++ "." ++ P.ind_name oib in
-       print_ty_name ind_name;;
+       let ind_ml_name := get_ty_name ind_name in
+       append ind_ml_name;;
 
        (* Print type args *)
        monad_fold_left (fun _ name => append (" " ++ name)) ty_arg_names tt;;
@@ -699,35 +715,40 @@ Definition print_mutual_inductive_body
 
        pop_indent;;
 
-       print_ind_bodies l false
-     end) (ind_bodies mib) true;;
+       print_ind_bodies l false ((ind_name, ind_ml_name) :: names)
+     end) (ind_bodies mib) true [];;
 
-  pop_indent.
+  pop_indent;;
+
+  ret names.
 
 Definition print_global_decl
            (name : kername)
-           (decl : Ex.global_decl) : PrettyPrinter unit :=
+           (decl : Ex.global_decl) : PrettyPrinter (list (kername * string)) :=
   match decl with
-  | Ex.ConstantDecl cst => print_constant_body name cst
-  | Ex.InductiveDecl mib => print_mutual_inductive_body name mib
+  | Ex.ConstantDecl cst => ml_name <- print_constant_body name cst;;
+                           ret [(name, ml_name)]
+  | Ex.InductiveDecl mib _ => print_mutual_inductive_body name mib
   end.
 
-Definition print_env : PrettyPrinter unit :=
+Definition print_env : PrettyPrinter (list (kername * string)) :=
   sig_col <- get_current_line_length;;
   push_indent sig_col;;
 
-  (fix f (l : Ex.global_env) (first : bool) :=
+  names <- (fix f (l : Ex.global_env) (first : bool) (names : list (kername * string)) :=
      match l with
+     | [] => ret names
      | (name, decl) :: l =>
 
        (if first then ret tt else (append_nl;; append_nl_and_indent));;
-       print_global_decl name decl;;
+       new_names <- print_global_decl name decl;;
 
-       f l false
-     | [] => ret tt
-     end) Σ true;;
+       f l false (new_names ++ names)%list
+     end) Σ true [];;
 
-  pop_indent.
+  pop_indent;;
+
+  ret names.
 End FixExEnv.
 
 Definition string_of_env_error Σ e :=
@@ -751,16 +772,81 @@ Definition wrap_typing_result {A} (Σ : P.global_env) (tr : typing_result A) : P
     printer_fail ("TypeError: " ++ string_of_type_error (P.empty_ext Σ) te)
   end.
 
-Axiom assump : string -> forall {A}, A.
+Definition wrap_option {A} (o : option A) (err : string) : PrettyPrinter A :=
+  match o with
+  | Some a => ret a
+  | None => printer_fail err
+  end.
 
-Lemma wf_empty_ext (Σ : P.global_env) :
-  ∥PT.wf Σ∥ -> ∥PT.wf_ext (P.empty_ext Σ)∥.
-Proof.
-  intros [wfΣ].
-  constructor.
-  split; [assumption|].
-  todo "on_udecl on empty_ext".
-Qed.
+(* Remove all generalization over ChainBase *)
+Fixpoint concretize_aux (cb_arg : nat) (t : E.term) : PrettyPrinter E.term :=
+    match t with
+    | E.tBox _ => ret t
+    | E.tRel n =>
+      if (n =? cb_arg)%nat then
+        printer_fail "term contains unhandled use of ChainBase"
+      else
+        ret t
+    | E.tVar _ => ret t
+    | E.tEvar n ts =>
+      ts <- monad_map (concretize_aux cb_arg) ts;;
+      ret (E.tEvar n ts)
+    | E.tLambda name t =>
+      t <- concretize_aux (S cb_arg) t;;
+      ret (E.tLambda name t)
+    | E.tLetIn name val body =>
+      val <- concretize_aux cb_arg val;;
+      body <- concretize_aux (S cb_arg) body;;
+      ret (E.tLetIn name val body)
+    | E.tApp (E.tConst _ as head) (E.tRel i) =>
+      if (i =? cb_arg)%nat then
+        ret head
+      else
+        ret t
+    | E.tApp head arg =>
+      head <- concretize_aux cb_arg head;;
+      arg <- concretize_aux cb_arg arg;;
+      ret (E.tApp head arg)
+    | E.tConst _ => ret t
+    | E.tConstruct _ _ => ret t
+    | E.tCase ind disc brs =>
+      disc <- concretize_aux cb_arg disc;;
+      brs <- monad_map (fun '(arity, body) => body <- concretize_aux cb_arg body;;
+                                              ret (arity, body)) brs;;
+      ret (E.tCase ind disc brs)
+    | E.tProj proj body =>
+      body <- concretize_aux cb_arg body;;
+      ret (E.tProj proj body)
+    | E.tFix defs i =>
+      let cb_arg := (List.length defs + cb_arg)%nat in
+      defs <- monad_map (fun d =>
+                           dbody <- concretize_aux cb_arg (dbody d);;
+                           ret {| dname := dname d;
+                                  dbody := dbody;
+                                  rarg := rarg d |}) defs;;
+      ret (E.tFix defs i)
+    | E.tCoFix defs i =>
+      let cb_arg := (List.length defs + cb_arg)%nat in
+      defs <- monad_map (fun d =>
+                           dbody <- concretize_aux cb_arg (dbody d);;
+                           ret {| dname := dname d;
+                                  dbody := dbody;
+                                  rarg := rarg d |}) defs;;
+      ret (E.tFix defs i)
+    end.
+
+Definition concretize (type : P.term) (body : E.term) : PrettyPrinter (P.term * E.term) :=
+  match type, body with
+  | P.tProd _ (P.tInd ind _) it, E.tLambda _ ib =>
+    if inductive_mind ind =? "ConCert.Execution.Blockchain.ChainBase" then
+      ib <- concretize_aux 0 ib;;
+      ret (it, ib)
+    else
+      ret (type, body)
+  | _, _ => ret (type, body)
+  end.
+
+Axiom assump : string -> forall {A}, A.
 
 Lemma proj_wf
       {Σ : P.global_env_ext}
@@ -774,25 +860,106 @@ Definition erase_and_debox_single
   match decl with
   | P.ConstantDecl cst =>
     let (type, body, _) := cst in
-    ebody <- match body with
-             | None => ret None
-             | Some body =>
-               ebody <- wrap_typing_result
-                          Σ.1
-                          (EF.erase Σ wfΣ [] body (assump "assuming well-typedness"));;
-               result <- wrap_EnvCheck (check_applied Σ.1 ebody (proj_wf wfΣ));;
-               if result then
-                 ret (Some (debox_all ebody))
-               else
-                 printer_fail "Not all constructors or constants are appropriately applied"
-             end;;
-    ret (Ex.ConstantDecl {| Ex.cst_type := type; Ex.cst_body := ebody |})
+    match body with
+    | None => ret (Ex.ConstantDecl {| Ex.cst_type := type; Ex.cst_body := None |})
+    | Some body =>
+      ebody <- wrap_typing_result
+                 Σ.1
+                 (EF.erase Σ wfΣ [] body (assump "assuming well-typedness"));;
+      result <- wrap_EnvCheck (check_applied Σ.1 ebody (proj_wf wfΣ));;
+      if result then
+        let ebody := debox_top_level (debox_all ebody) in
+        '(type, ebody) <- concretize type ebody;;
+        ret (Ex.ConstantDecl {| Ex.cst_type := type; Ex.cst_body := Some ebody |})
+      else
+        printer_fail "Not all constructors or constants are appropriately applied"
+    end
   | P.InductiveDecl mib =>
-    (*mib <- wrap_typing_result
-             Σ.1
-             (EF.erase_mutual_inductive_body Σ wfΣ mib);;*)
-    ret (Ex.InductiveDecl mib)
+    emib <- wrap_typing_result
+              Σ.1
+              (EF.erase_mutual_inductive_body Σ wfΣ mib);;
+    ret (Ex.InductiveDecl mib emib)
   end.
+
+Definition ignored_concert_types :=
+  ["ConCert.Execution.Blockchain.ChainBase";
+   "ConCert.Execution.Blockchain.Chain";
+   "ConCert.Execution.Blockchain.ContractCallContext";
+   "ConCert.Extraction.MidlangExtract.extraction_chain_base"].
+
+Lemma wf_empty_ext (Σ : P.global_env) :
+  ∥PT.wf Σ∥ -> ∥PT.wf_ext (P.empty_ext Σ)∥.
+Proof.
+  intros [wfΣ].
+  constructor.
+  split; [assumption|].
+  todo "on_udecl on empty_ext".
+Qed.
+
+Definition add_seen (n : kername) (seen : list kername) : list kername :=
+  if existsb (String.eqb n) seen then
+    seen
+  else
+    n :: seen.
+
+Fixpoint term_deps
+         (seen : list kername)
+         (t : term) : list kername :=
+  match t with
+  | tEvar _ ts => fold_left term_deps ts seen
+  | tLambda _ t => term_deps seen t
+  | tLetIn _ t1 t2
+  | tApp t1 t2 => term_deps (term_deps seen t1) t2
+  | tConst n => add_seen n seen
+  | tConstruct ind _ => add_seen (inductive_mind ind) seen
+  | tCase (ind, _) t brs =>
+    let seen := term_deps (add_seen (inductive_mind ind) seen) t in
+    fold_left (fun seen '(_, t) => term_deps seen t) brs seen
+  | tProj (ind, _, _) t => term_deps (add_seen (inductive_mind ind) seen) t
+  | tFix defs _
+  | tCoFix defs _ =>
+    fold_left (fun seen d => term_deps seen (dbody d)) defs seen
+  | _ => seen
+  end.
+
+Definition decl_deps (decl : Ex.global_decl) : list kername :=
+  match decl with
+  | Ex.ConstantDecl body =>
+    match Ex.cst_body body with
+    | Some body => term_deps [] body
+    | None => []
+    end
+  | Ex.InductiveDecl _ emib =>
+    let one_inductive_body_deps seen oib :=
+        let seen := fold_left (fun seen '(_, t, _) => term_deps seen t) (ind_ctors oib) seen in
+        fold_left (fun seen '(_, t) => term_deps seen t) (ind_projs oib) seen in
+
+    fold_left one_inductive_body_deps (ind_bodies emib) []
+  end.
+
+(* Return all recursive dependencies in topological order of the specified seed declarations *)
+Definition decl_deps_recursive
+           (Σ : Ex.global_env)
+           (seeds : list kername)
+           (ignore : list kername) : option (list (kername * Ex.global_decl)) :=
+  let fix go n seen name :=
+      match n with
+      | 0 => None
+      | S n =>
+        if (existsb (String.eqb name) ignore ||
+            if Ex.lookup_env seen name then true else false)%bool then
+          ret seen
+        else
+          match Ex.lookup_env Σ name with
+          | Some decl =>
+            let seen := (name, decl) :: seen in
+            let deps := decl_deps decl in
+            monad_fold_left (go n) deps seen
+          | None =>
+            None
+          end
+      end in
+  monad_fold_left (go (N.to_nat 10000)) seeds [].
 
 (* Extract the specified environment to Midlang, creating definitions for all symbols. *)
 Definition extract_env (Σ : T.global_env) : PrettyPrinter unit :=
@@ -822,8 +989,15 @@ Definition extract_env (Σ : T.global_env) : PrettyPrinter unit :=
   Σex <- monad_map (fun '(name, decl) =>
                       decl <- erase_and_debox_single Σext wfΣext decl;;
                       ret (name, decl)) Σ;;
-  print_env Σex.
+  let seeds := ["ConCert.Extraction.MidlangExtract.init";
+                "ConCert.Extraction.MidlangExtract.receive"] in
+  to_extract <- wrap_option (decl_deps_recursive Σex seeds ignored_concert_types)
+                            "Ran out of fuel while fetching dependencies";;
+  (*monad_fold_left (fun _ '(name, _) => append name;; append_nl) to_extract tt;;*)
+  print_env to_extract;;
+  ret tt.
 
+(*
 Local Open Scope nat.
 
 Inductive Msg :=
@@ -844,7 +1018,7 @@ Definition test : nat :=
   let x := 5 in
   let foo n := S n in
   let even :=
-      fix even n :=
+      fix even n :
         match n with
         | 0 => true
         | S n => odd n
@@ -868,8 +1042,24 @@ Definition test' : bool :=
   let x := let y := true in y in
   let y := x in y.
 
+Definition list_debruijn := fold_right (fun b a => b) 0 [].
+  (*(fun (x : list nat) =>
+     match x with
+     | nil => nil
+     | y :: ys => x
+     end).*)
+
+Definition fun_fix {A} (f : nat -> A -> A) (a : A) :=
+  fix g (l : list nat) : A :=
+    match l with
+    | [] => a
+    | n :: l => f n (g l)
+    end.
+
 (*Quote Recursively Definition test_program := test.*)
-Quote Recursively Definition test_program := recv.
+(*Quote Recursively Definition test_program := (init; recv).*)
+(*Quote Recursively Definition test_program := list_debruijn.*)
+(*Quote Recursively Definition test_program := fun_fix.*)
 
 Local Open Scope string.
 Definition test3 :=
@@ -878,7 +1068,11 @@ Definition test3 :=
   | inr (_, output) => output
   end.
 
-Compute test3.
+Definition foo' := fun x => x = 5.
+
+Quote Recursively Definition aaa := (fun x => x = 5).
+
+Compute erase_template_program aaa.
 
 Compute erase_check_debox_all_print [] "foo" [] test_program.
 
@@ -895,3 +1089,144 @@ Definition test2 : string :=
   end.
 
 Compute test2.
+*)
+
+From Coq Require Import ZArith.
+
+Section Counter.
+Context `{ChainBase}.
+Inductive Msg :=
+| increment
+| decrement.
+
+Global Instance Serializable_Msg : Serializable Msg :=
+  Derive Serializable Msg_rect<increment, decrement>.
+
+Local Open Scope Z.
+Definition t37 := 37%Z.
+Definition t237 := 237%Z.
+Definition test := (t37 + t237 =? 274)%Z.
+Definition init
+           (chain : Chain)
+           (ctx : ContractCallContext)
+           (setup : unit) : option Z :=
+  Some (if test then 0 else 0)%Z.
+
+Definition receive
+           (chain : Chain)
+           (ctx : ContractCallContext)
+           (state : Z)
+           (maybe_msg : option Msg)
+  : option (Z * list ActionBody) :=
+  match maybe_msg with
+  | Some increment => Some (state + 1, [])
+  | Some decrement => Some (state - 1, [])
+  | _ => None
+  end.
+
+Program Definition contract : Contract unit Msg Z :=
+  {| Blockchain.init := init; Blockchain.receive := receive; |}.
+
+End Counter.
+
+Local Open Scope nat.
+
+(*
+Fixpoint erasable_program (name : qualid) : TemplateMonad program :=
+  cst <- tmQuoteConstant name false;;
+  let body := cst_body cst in
+  match body with
+  | None => tmFail ("cannot get body of constant " ++ name)
+  | Some body =>
+    (fix aux (tries : nat) (env : global_env) : TemplateMonad program :=
+    match tries with
+    | 0 => tmFail "out of fuel"
+    | S tries =>
+      let p := (env, body) in
+      result <- tmEval lazy (check_applied p);;
+      match result with
+      | CorrectDecl _ => ret p
+      | EnvError Σ (IllFormedDecl _ e)  =>
+        match e with
+        | UndeclaredConstant c =>
+          tmMsg ("need constant " ++ c);;
+          cst <- tmQuoteConstant c false;;
+          let cst := {| cst_type := cst_type cst;
+                        cst_body := None;
+                        cst_universes :=
+                          Monomorphic_ctx (LevelSetProp.of_list [], ConstraintSet.empty); |} in
+          let env := List.filter (fun '(n, _) => negb (n =? c)%string) env in
+          aux tries ((c, ConstantDecl cst) :: env)
+        | UndeclaredInductive c
+        | UndeclaredConstructor c _ =>
+          let name := inductive_mind c in
+          tmMsg ("need inductive " ++ name);;
+          ind <- tmQuoteInductive name;;
+          let ind := {| ind_finite := ind_finite ind;
+                        ind_npars := ind_npars ind;
+                        ind_params := ind_params ind;
+                        ind_bodies := ind_bodies ind;
+                        ind_universes :=
+                          Monomorphic_ctx (LevelSetProp.of_list [], ConstraintSet.empty);
+                        ind_variance := ind_variance ind |} in
+          let env := List.filter (fun '(n, _) => negb (n =? name)%string) env in
+          aux tries ((name, InductiveDecl ind) :: env)
+        | _ =>
+          tmFail (string_of_type_error Σ e)
+        end
+      | EnvError Σ (AlreadyDeclared id) =>
+        tmFail ("Already declared: " ++ id)
+      end
+    end) 1000 []
+  end.
+
+Definition erase_and_print p : TemplateMonad unit :=
+  match erase_and_print_template_program p with
+  | inl s => tmMsg s
+  | inr s => tmMsg s
+  end.
+*)
+
+Import T.
+Definition extract_def_name {A : Type} (a : A) : TemplateMonad qualid :=
+  a <- tmEval cbn a;;
+  quoted <- tmQuote a;;
+  let (head, args) := TUtil.decompose_app quoted in
+  match head with
+  | tConst name _ => ret name
+  | _ => tmFail ("Expected constant at head, got " ++ TUtil.string_of_term head)
+  end.
+
+(*Quote Recursively Definition test_program := (@contract extraction_chain_base).*)
+
+Quote Recursively Definition test_program := (init, receive).
+
+(*
+*)
+
+Definition extracted :=
+  match finish_print (append_nl;; extract_env test_program.1) with
+  | inl err => ("Printer error: " ++ err)%string
+  | inr (_, output) => output
+  end.
+
+Compute extracted.
+
+Definition toMidlang
+           {Setup Msg State}
+           `{Serializable Setup}
+           `{Serializable Msg}
+           `{Serializable State}
+           (contract : forall (cb : ChainBase), Contract Setup Msg State) : TemplateMonad unit :=
+  init_name <- extract_def_name (Blockchain.init (contract extraction_chain_base));;
+  receive_name <- extract_def_name (Blockchain.receive (contract extraction_chain_base));;
+  x <- erasable_program receive_name;;
+  tmMsg (string_of_term x.2).
+
+Run TemplateProgram (toMidlang (fun cb => @contract cb)).
+
+Definition test : TemplateProgram unit :=
+  tmEval
+
+Definition foo (m : FMap nat nat) : option nat :=
+  FMap.find 3 m.
